language/move-prover/tests/sources/functional/emits.move
@@ -31,6 +31,56 @@ module TestEmits {
     }
 
 
+    // ---------------
+    // multiple events
+    // ---------------
+
+    public fun multiple(handle: &mut EventHandle<DummyEvent>) {
+        Event::emit_event(handle, DummyEvent{msg: 0});
+        Event::emit_event(handle, DummyEvent{msg: 1});
+    }
+    spec fun multiple {
+        emits DummyEvent{msg: 0} to handle;
+        emits DummyEvent{msg: 1} to handle;
+    }
+
+    public fun multiple_incorrect(handle: &mut EventHandle<DummyEvent>) {
+        Event::emit_event(handle, DummyEvent{msg: 0});
+        Event::emit_event(handle, DummyEvent{msg: 1});
+    }
+    spec fun multiple_incorrect {
+        emits DummyEvent{msg: 0} to handle;
+        emits DummyEvent{msg: 1} to handle;
+        emits DummyEvent{msg: 2} to handle;
+    }
+
+    public fun multiple_same(handle: &mut EventHandle<DummyEvent>) {
+        Event::emit_event(handle, DummyEvent{msg: 0});
+        Event::emit_event(handle, DummyEvent{msg: 0});
+    }
+    spec fun multiple_same {
+        emits DummyEvent{msg: 0} to handle;
+        emits DummyEvent{msg: 0} to handle;
+    }
+
+    public fun multiple_same_incorrect(handle: &mut EventHandle<DummyEvent>) {
+        Event::emit_event(handle, DummyEvent{msg: 0});
+    }
+    spec fun multiple_same_incorrect {
+        emits DummyEvent{msg: 0} to handle;
+        emits DummyEvent{msg: 0} to handle;
+    }
+
+    public fun multiple_different_handle(handle: &mut EventHandle<DummyEvent>, handle2: &mut EventHandle<DummyEvent>) {
+        Event::emit_event(handle, DummyEvent{msg: 0});
+        Event::emit_event(handle2, DummyEvent{msg: 0});
+    }
+    spec fun multiple_different_handle {
+        emits DummyEvent{msg: 0} to handle;
+        emits DummyEvent{msg: 0} to handle2;
+    }
+
+
     // ------------------------------
     // conditional `emits` statements
     // ------------------------------
@@ -59,6 +109,75 @@ module TestEmits {
         }
     }
     spec fun conditional_missing_condition_incorrect {
+        emits DummyEvent{msg: 0} to handle;
+    }
+
+    public fun conditional_bool(b: bool, handle: &mut EventHandle<DummyEvent>) {
+        if (b) {
+            Event::emit_event(handle, DummyEvent{msg: 0});
+        }
+    }
+    spec fun conditional_bool {
+        emits DummyEvent{msg: 0} to handle if b;
+    }
+
+    public fun conditional_multiple(b0: bool, b1: bool, b2: bool, handle: &mut EventHandle<DummyEvent>) {
+        if (b0) {
+            Event::emit_event(handle, DummyEvent{msg: 0});
+        };
+        if (b1) {
+            Event::emit_event(handle, DummyEvent{msg: 1});
+        };
+        if (b2) {
+            Event::emit_event(handle, DummyEvent{msg: 2});
+        }
+    }
+    spec fun conditional_multiple {
+        emits DummyEvent{msg: 0} to handle if b0;
+        emits DummyEvent{msg: 1} to handle if b1;
+        emits DummyEvent{msg: 2} to handle if b2;
+    }
+
+    public fun conditional_multiple_incorrect(b: bool, handle: &mut EventHandle<DummyEvent>) {
+        Event::emit_event(handle, DummyEvent{msg: 0});
+        Event::emit_event(handle, DummyEvent{msg: 1});
+        if (b) {
+            Event::emit_event(handle, DummyEvent{msg: 2});
+        }
+    }
+    spec fun conditional_multiple_incorrect {
+        emits DummyEvent{msg: 0} to handle;
+        emits DummyEvent{msg: 1} to handle;
+        emits DummyEvent{msg: 2} to handle;
+    }
+
+    public fun conditional_multiple_same(b0: bool, b1: bool, b2: bool, handle: &mut EventHandle<DummyEvent>) {
+        if (b0) {
+            Event::emit_event(handle, DummyEvent{msg: 0});
+        };
+        if (b1) {
+            Event::emit_event(handle, DummyEvent{msg: 0});
+        };
+        if (b2) {
+            Event::emit_event(handle, DummyEvent{msg: 0});
+        }
+    }
+    spec fun conditional_multiple_same {
+        emits DummyEvent{msg: 0} to handle if b0;
+        emits DummyEvent{msg: 0} to handle if b1;
+        emits DummyEvent{msg: 0} to handle if b2;
+    }
+
+    public fun conditional_multiple_same_incorrect(b: bool, handle: &mut EventHandle<DummyEvent>) {
+        Event::emit_event(handle, DummyEvent{msg: 0});
+        Event::emit_event(handle, DummyEvent{msg: 0});
+        if (b) {
+            Event::emit_event(handle, DummyEvent{msg: 0});
+        }
+    }
+    spec fun conditional_multiple_same_incorrect {
+        emits DummyEvent{msg: 0} to handle;
+        emits DummyEvent{msg: 0} to handle;
         emits DummyEvent{msg: 0} to handle;
     }
 
